\begin{equation}
C_m = C_{m_0} + C_{m_\alpha}\alpha + C_{m_{i_H}} i_H
\label{eq_cmWithH}
\end{equation}
Now define every parameter in equation \ref{eq_cmWithH}.
$$C_{m_0} = C_{m_{ac_{wb}}} + C_{L_{0_{wb}}}(\bar x_{cg} - \bar x_{ac_{wb}})$$
$$C_{m_\alpha} = C_{L_{\alpha_{wb}}}(\bar x_{cg} - \bar x_{ac_{wb}})-
C_{L_{\alpha_{H}}}\eta_H
\dfrac{S_H}{S}
(1-\dfrac{\partial \varepsilon}{\partial \alpha})
(\bar x_{ac_{H}}-\bar x_{cg})
$$
$$C_{m_{i_H}} = C_{L_{\alpha_{H}}}\eta_H
\dfrac{S_H}{S}
(\bar x_{ac_{H}}-\bar x_{cg})$$
Data:
$$\alpha = 7.88^{\circ},\quad C_{m_{ac_{wb}}} = -0.032,\quad C_{L_{\alpha_{wb}}}= 0.08
,\quad \bar x_{cg} = 0.35
,\quad \bar x_{ac} = 0.24
$$